use leap_size everywhere instead of old min

deps/poulet4/lib/P4automata/Bisimulations/Leaps.v
@@ -19,23 +19,24 @@ Section Leaps.
   Variable (a: p4automaton).
   Notation conf := (configuration a).
 
+  Definition leap_size (q1 q2: conf) : nat :=
+    match conf_state q1, conf_state q2 with
+    | inl s1, inl s2 => min (configuration_room_left q1) (configuration_room_left q2)
+    | inl s1, inr _ => configuration_room_left q1
+    | inr _, inl s2 => configuration_room_left q2
+    | inr _, inr _ => 1
+    end.
+
   Inductive close_interpolate (R: rel conf) : rel conf :=
     | InterpolateBase:
         forall q1 q2,
           R q1 q2 -> close_interpolate _ q1 q2
     | InterpolateStep
         (q1 q2: conf)
-        (s1 s2: states a)
-        (b: bool)
-        (H1: configuration_has_room q1)
-        (H2: configuration_has_room q2):
-        conf_state q1 = inl s1 ->
-        conf_state q2 = inl s2 ->
+        (b: bool):
         close_interpolate R q1 q2 ->
         (forall buf,
-            length buf = min
-              (configuration_room_left q1)
-              (configuration_room_left q2) ->
+            length buf = leap_size q1 q2 ->
             R (follow q1 buf) (follow q2 buf)) ->
         close_interpolate R (step q1 b) (step q2 b).
 
@@ -44,9 +45,7 @@ Section Leaps.
       forall q1 q2,
         (accepting q1 <-> accepting q2) ->
         (forall buf,
-          length buf = min
-            (configuration_room_left q1)
-            (configuration_room_left q2) ->
+          length buf = leap_size q1 q2 ->
           bisimilar_with_leaps (follow q1 buf) (follow q2 buf)) ->
         bisimilar_with_leaps q1 q2.
 
