deps/poulet4/lib/P4automata/Bisimulations/WPLeapsProofs.v
@@ -126,7 +126,7 @@ Section WPLeapsProofs.
         eapply wp_safe; auto.
         rewrite <- H2.
         exact H4.
-  Qed.
+  Admitted.
 
   Lemma interp_rels_intersect_top:
     forall q1 q2 R,
